$$T_{pq}(a, b) : 
\begin{cases}
a \leftarrow bq + aq + ap \\
b \leftarrow bp + aq
\end{cases}$$

$T_{pq}$를 두 번 적용하면 $a$와 $b$는 다음과 같이 변환된다.
$$
\begin{aligned}
T_{pq}(T_{pq}(a, b))
&= T_{pq}(bq + aq + ap, bp + aq) \\
&= ((bp + aq)q + (bq + aq + ap)q + (bq + aq + ap)p, (bp + aq)p + (bq + aq + ap)q) \\
&= (bpq + aq^2 + bq^2 + aq^2 + apq + bpq + apq + ap^2, bp^2 + apq + bq^2 + aq^2 + apq) \\
&= (b(2pq + q^2) + a(2pq + q^2) + a(q^2 + p^2), b(p^2 + q^2) + a(2pq + q^2)) \\
&= (bq^\prime + aq^\prime + ap^\prime, bp^\prime + aq^\prime)
\end{aligned}
$$

따라서, $p^\prime = p^2 + q^2$, $q^\prime = 2pq + q^2$이다.

```javascript
function fib(n) {
    return fib_iter(1, 0, 0, 1, n);
}

function fib_iter(a, b, p, q, count) {
    return count === 0
           ? b
           : is_even(count)
           ? fib_iter(a,
                      b,
                      p * p + q * q,
                      2 * p * q + q * q,
                      count / 2)
           : fib_iter(b * q + a * q + a * p,
                      b * p + a * q,
                      p,
                      q,
                      count - 1);
}
```